extending list model
Signed-off-by: Roni Häcki <roni.haecki@inf.ethz.ch>

CleanQ/CleanQ_ListModel.thy
@@ -15,7 +15,10 @@
 section "CleanQ Abstract List Model"
 
 text \<open>
-  We define
+  We define a first refinement of the abstract model based on sets. We redefine the
+  transfer sets as lists in order to get the FIFO for the transfer from X to Y and
+  vice versa. We define the model of this first refinement in the the following 
+  Isabelle theory: 
 \<close>
 
 theory CleanQ_ListModel
@@ -24,13 +27,137 @@ theory CleanQ_ListModel
 (*>*)
 begin
 
-
-
 (* ==================================================================================== *)
 subsection \<open>State Definition\<close>
 (* ==================================================================================== *)
+text \<open>
+  The model is similar to the set model except the change of the transfer sets.
+
+  \<^item> TXY: this is a list of buffers in transfer from X to Y.
+  \<^item> TYX: this is a list of buffers in transfer from Y to X.
+\<close>
+
+record 'a CleanQ_List_State =
+  lSX  :: "'a set"
+  lSY  :: "'a set"
+  lTXY :: "'a list"
+  lTYX :: "'a list"
+
+(* ==================================================================================== *)
+subsection \<open>CleanQ List Model Invariants\<close>
+(* ==================================================================================== *)
+
+(* ------------------------------------------------------------------------------------ *)
+subsubsection \<open>Images of the previously defined invariants\<close>
+(* ------------------------------------------------------------------------------------ *)
+
+text \<open>The union of all sets is constant. Image for \verb+CleanQ_List+\<close>
+fun I1_img :: "'a CleanQ_List_State \<Rightarrow> 'a set \<Rightarrow> bool"
+  where "I1_img rb K \<longleftrightarrow> ((lSX rb) \<union> (lSY rb) \<union> set (lTXY rb) \<union> set (lTYX rb)) = K"
+
+text \<open>All pairwise intersections are empty. Image for \verb+CleanQ_List+.\<close>
+fun I2_img :: "'a CleanQ_List_State \<Rightarrow> bool"
+  where "I2_img rb \<longleftrightarrow> lSX rb \<inter> lSY rb = {} \<and> lSX rb \<inter> set (lTXY rb) = {} \<and> lSX rb \<inter> set (lTYX rb) = {} \<and> 
+    lSY rb \<inter> set (lTXY rb) = {} \<and> lSY rb \<inter> set (lTYX rb) = {} \<and> 
+    set (lTXY rb) \<inter> set (lTYX rb) = {}"
+
+(* ------------------------------------------------------------------------------------ *)
+subsubsection \<open>I3: the elements in the transfer lists are distinct\<close>
+(* ------------------------------------------------------------------------------------ *)
+
+text \<open>This invariant is required for the move from sets to lists. In sets an element
+      occurs only once while in lists it can occur multiple times. If we map the
+      list which contains twice the same element, it would be mapped to only
+      a single set element. In order to avoid this the elements of the lists need
+     to be distinct\<close>
+fun I3 :: "'a CleanQ_List_State \<Rightarrow> bool"
+  where "I3 st_list \<longleftrightarrow> distinct (lTXY st_list @ lTYX st_list)"
+
+(* ------------------------------------------------------------------------------------ *)
+subsubsection \<open>CleanQ List Invariants\<close>
+(* ------------------------------------------------------------------------------------ *)
+
+text \<open>
+  We combine all invariants for the abstract CleanQ list model and define the predicate 
+  \verb+CleanQ_List_Invariants+.
+\<close>
+
+fun CleanQ_List_Invariants :: "'a set \<Rightarrow> 'a CleanQ_List_State \<Rightarrow> bool"
+  where "CleanQ_List_Invariants K rb \<longleftrightarrow> I1_img rb K \<and> I2_img rb \<and> I3 rb"
 
 
-subsubsection \<open>Abstract Queue Definition\<close>
+
+(* ==================================================================================== *)
+subsection \<open>State Transition Operations\<close>
+(* ==================================================================================== *)
+
+text \<open>
+  The two agents can, independently from each other, perform one of two operations, 
+  \verb+enqueue+ and \verb+dequeue+,  which trigger an ownership transfer of buffer 
+  elements.  
+\<close>
+
+(* ------------------------------------------------------------------------------------ *)
+subsubsection \<open>Enqueue Operation\<close>
+(* ------------------------------------------------------------------------------------ *)
+
+text \<open>
+  The enqueue operation is analogous to the Set operations except that the elements
+  are added to the end of the queue instead of simply added to the set. 
+\<close>
+
+definition CleanQ_List_enq_x :: "'a \<Rightarrow> 'a CleanQ_List_State  \<Rightarrow> 'a CleanQ_List_State"
+  where "CleanQ_List_enq_x b rb = rb  \<lparr>  lSX := (lSX rb) - {b},  lTXY := (lTXY rb @ [b]) \<rparr>"
+
+definition CleanQ_List_enq_y :: "'a \<Rightarrow> 'a CleanQ_List_State  \<Rightarrow> 'a CleanQ_List_State"
+  where "CleanQ_List_enq_y b rb = rb  \<lparr>  lSY := (lSY rb) - {b},  lTYX := (lTYX rb @ [b]) \<rparr>"
+
+text \<open>
+  These definitions are the same as producing a new record:
+\<close>
+lemma CleanQ_List_enq_x_upd :
+  "CleanQ_List_enq_x b rb = \<lparr> lSX = (lSX rb) - {b},  lSY = (lSY rb), 
+                             lTXY = (lTXY rb) @ [b],  lTYX = (lTYX rb) \<rparr>"
+  by(simp add:CleanQ_List_enq_x_def)
+
+lemma CleanQ_List_enq_y_upd :
+  "CleanQ_List_enq_y b rb = \<lparr> lSX = (lSX rb), lSY = (lSY rb) - {b}, 
+                             lTXY = (lTXY rb), lTYX = (lTYX rb) @ [b] \<rparr>"
+  by(simp add:CleanQ_List_enq_y_def)
+
+
+(* ------------------------------------------------------------------------------------ *)
+subsubsection \<open>Dequeue Operation\<close>
+(* ------------------------------------------------------------------------------------ *)
+
+
+text \<open>
+  The dequeue operation is analogous to the Set operations except that the elements
+  are removed from the head of the queue instead of simply removed to the set. 
+\<close>
+
+definition CleanQ_List_deq_x :: "'a \<Rightarrow> 'a CleanQ_List_State  \<Rightarrow> 'a CleanQ_List_State"
+  where "CleanQ_List_deq_x b rb = \<lparr> lSX = (lSX rb) \<union> {b}, lSY = (lSY rb), lTXY = (lTXY rb),  
+                                   lTYX = (remove1 b (lTYX rb)) \<rparr>"
+
+definition CleanQ_List_deq_y :: "'a \<Rightarrow> 'a CleanQ_List_State  \<Rightarrow> 'a CleanQ_List_State"
+  where "CleanQ_List_deq_y b rb = \<lparr> lSX = (lSX rb),  lSY = (lSY rb) \<union> {b}, 
+                                   lTXY = (remove1 b (lTXY rb)),  lTYX = (lTYX rb) \<rparr>"
+
+
+text \<open>
+  These definitions are the same as producing a new record:
+\<close>
+
+lemma CleanQ_List_deq_x_upd :
+  "CleanQ_List_deq_x b rb = \<lparr> lSX = (lSX rb) \<union> {b},  lSY = (lSY rb), 
+                             lTXY = (lTXY rb), lTYX = remove1 b (lTYX rb) \<rparr>"
+  by(simp add:CleanQ_List_deq_x_def)
+
+lemma CleanQ_List_deq_y_upd :
+  "CleanQ_List_deq_y b rb = \<lparr> lSX = (lSX rb),  lSY = (lSY rb) \<union> {b},
+                             lTXY = remove1 b (lTXY rb),  lTYX = (lTYX rb) \<rparr>"
+  by(simp add:CleanQ_List_deq_y_def)
+
 
 end
